DynamoDbEncryptionMiddlewareInternal/runtimes/java/src/main/smithy-generated/software/amazon/cryptography/dynamoDbEncryption/model/Insert.java
@@ -1,0 +1,61 @@
+// Copyright Amazon.com Inc. or its affiliates. All Rights Reserved.
+// SPDX-License-Identifier: Apache-2.0
+// Do not modify this file. This file is machine generated, and any changes to it will be overwritten.
+package software.amazon.cryptography.dynamoDbEncryption.model;
+
+import java.util.Objects;
+
+public class Insert {
+  private final String string;
+
+  protected Insert(BuilderImpl builder) {
+    this.string = builder.string();
+  }
+
+  public String string() {
+    return this.string;
+  }
+
+  public Builder toBuilder() {
+    return new BuilderImpl(this);
+  }
+
+  public static Builder builder() {
+    return new BuilderImpl();
+  }
+
+  public interface Builder {
+    Builder string(String string);
+
+    String string();
+
+    Insert build();
+  }
+
+  static class BuilderImpl implements Builder {
+    protected String string;
+
+    protected BuilderImpl() {
+    }
+
+    protected BuilderImpl(Insert model) {
+      this.string = model.string();
+    }
+
+    public Builder string(String string) {
+      this.string = string;
+      return this;
+    }
+
+    public String string() {
+      return this.string;
+    }
+
+    public Insert build() {
+      if (Objects.isNull(this.string()))  {
+        throw new IllegalArgumentException("Missing value for required field `string`");
+      }
+      return new Insert(this);
+    }
+  }
+}
