DynamoDbEncryptionMiddlewareInternal/runtimes/java/src/main/smithy-generated/software/amazon/cryptography/dynamoDbEncryption/model/Substring.java
@@ -1,0 +1,84 @@
+// Copyright Amazon.com Inc. or its affiliates. All Rights Reserved.
+// SPDX-License-Identifier: Apache-2.0
+// Do not modify this file. This file is machine generated, and any changes to it will be overwritten.
+package software.amazon.cryptography.dynamoDbEncryption.model;
+
+import java.util.Objects;
+
+public class Substring {
+  private final Integer low;
+
+  private final Integer high;
+
+  protected Substring(BuilderImpl builder) {
+    this.low = builder.low();
+    this.high = builder.high();
+  }
+
+  public Integer low() {
+    return this.low;
+  }
+
+  public Integer high() {
+    return this.high;
+  }
+
+  public Builder toBuilder() {
+    return new BuilderImpl(this);
+  }
+
+  public static Builder builder() {
+    return new BuilderImpl();
+  }
+
+  public interface Builder {
+    Builder low(Integer low);
+
+    Integer low();
+
+    Builder high(Integer high);
+
+    Integer high();
+
+    Substring build();
+  }
+
+  static class BuilderImpl implements Builder {
+    protected Integer low;
+
+    protected Integer high;
+
+    protected BuilderImpl() {
+    }
+
+    protected BuilderImpl(Substring model) {
+      this.low = model.low();
+      this.high = model.high();
+    }
+
+    public Builder low(Integer low) {
+      this.low = low;
+      return this;
+    }
+
+    public Integer low() {
+      return this.low;
+    }
+
+    public Builder high(Integer high) {
+      this.high = high;
+      return this;
+    }
+
+    public Integer high() {
+      return this.high;
+    }
+
+    public Substring build() {
+      if (Objects.isNull(this.low()))  {
+        throw new IllegalArgumentException("Missing value for required field `low`");
+      }
+      return new Substring(this);
+    }
+  }
+}
