DynamoDbEncryptionMiddlewareInternal/runtimes/java/src/main/smithy-generated/software/amazon/cryptography/dynamoDbEncryption/model/Suffix.java
@@ -1,0 +1,64 @@
+// Copyright Amazon.com Inc. or its affiliates. All Rights Reserved.
+// SPDX-License-Identifier: Apache-2.0
+// Do not modify this file. This file is machine generated, and any changes to it will be overwritten.
+package software.amazon.cryptography.dynamoDbEncryption.model;
+
+import java.util.Objects;
+
+public class Suffix {
+  private final int length;
+
+  protected Suffix(BuilderImpl builder) {
+    this.length = builder.length();
+  }
+
+  public int length() {
+    return this.length;
+  }
+
+  public Builder toBuilder() {
+    return new BuilderImpl(this);
+  }
+
+  public static Builder builder() {
+    return new BuilderImpl();
+  }
+
+  public interface Builder {
+    Builder length(int length);
+
+    int length();
+
+    Suffix build();
+  }
+
+  static class BuilderImpl implements Builder {
+    protected int length;
+
+    protected BuilderImpl() {
+    }
+
+    protected BuilderImpl(Suffix model) {
+      this.length = model.length();
+    }
+
+    public Builder length(int length) {
+      this.length = length;
+      return this;
+    }
+
+    public int length() {
+      return this.length;
+    }
+
+    public Suffix build() {
+      if (Objects.isNull(this.length()))  {
+        throw new IllegalArgumentException("Missing value for required field `length`");
+      }
+      if (Objects.nonNull(this.length()) && this.length() < 1) {
+        throw new IllegalArgumentException("`length` must be greater than or equal to 1");
+      }
+      return new Suffix(this);
+    }
+  }
+}
